fix: define refinement of α × β properly, fix ConstantFold case study (#131)
This PR introduces a proper refinement relation for products α × β.
Previously, this implicitly used the fallback instance for refinement,
meaning refinement on the pair was defined via equality, even when
better refinement relations on `α` and `β` were available.

To avoid this issue happening again in the future, the default
refinement instance is no longer an instance, but now just a definition.

Further, this PR fixes the constant folding case study. The case study
was not properly adjusted after the core framework was moved to using
the equation invariant. The PR also adds the case study to the default
ProofSketch import, so that it should be built in CI, preventing future
regressions

EffectSSA/ProofSketch/Assumptions.lean
@@ -17,7 +17,7 @@ class SSA (ι : Type) (σ : outParam Type) (ν : outParam Type) : Type where
   [valRefine : Refinement ν]
   initialState : σ
   denoteInst : ι → σ → List ν → σ × List ν
-  isRefinedBy_denote :
+  isRefinedBy_denoteInst :
     s ⊒ t → xs ⊒ ys → denoteInst i s xs ⊒ denoteInst i t ys
 
 attribute [implicit_reducible, instance]
@@ -25,6 +25,10 @@ attribute [implicit_reducible, instance]
 
 @[reducible] instance SSA.instDenote [ssa : SSA ι σ ν] : Denote ι (σ → List ν → σ × List ν) where
   denote := ssa.denoteInst
+
+@[grind .] theorem SSA.isRefinedBy_denote [ssa : SSA ι σ ν] (i : ι) :
+    s ⊒ t → xs ⊒ ys → ⟦i⟧ s xs ⊒ ⟦i⟧ t ys :=
+  SSA.isRefinedBy_denoteInst
 
 /-!
 ## Environment
