EffectSSA/ProofSketch.lean
@@ -1,1 +1,2 @@
 import EffectSSA.ProofSketch.ProofSketch
+import EffectSSA.ProofSketch.CaseStudy.ConstFold
